src/RelationalTransferFunction.v
@@ -21,6 +21,12 @@ Class transfer_function_relational {abstract_state: eqType} {p: Program}
         le (transfer_inst inst (compose_relation comp_a a))
            (compose_relation comp_a (transfer_inst inst a));
 
+    transfer_inst_compose_transitive_closure :
+      forall inst a comp_a,
+        le (transfer_inst inst (compose_transitive_closure comp_a a))
+           (compose_transitive_closure comp_a (transfer_inst inst a));
+
+
     transfer_term : Term -> abstract_state -> list (abstract_state * bbid);
     transfer_term_sound :
       forall term R bb R',
@@ -36,5 +42,10 @@ Class transfer_function_relational {abstract_state: eqType} {p: Program}
     transfer_term_compose :
       forall term a a' comp_a bb,
         (a', bb) \in (transfer_term term (compose_relation comp_a a)) ->
-        exists a'', (a'', bb) \in transfer_term term a /\ le a' (compose_relation comp_a a'');
+                     exists a'', (a'', bb) \in transfer_term term a /\ le a' (compose_relation comp_a a'');
+
+    transfer_term_compose_transitive_closure :
+      forall term a a' comp_a bb,
+        (a', bb) \in (transfer_term term (compose_transitive_closure comp_a a)) ->
+                     exists a'', (a'', bb) \in transfer_term term a /\ le a' (compose_transitive_closure comp_a a'');
   }.
